added edge labeled RG

project/algebraic/algebraic_graph_to_RG.v
@@ -5,28 +5,28 @@ Require Import MyProject.project.relational_graph.
 
 
 (* Defining Conversion from Algebraic Graph to Record Graph *)
-Definition empty_RG {A : Type} : RG A.
+Definition RG_unlE_empty {A : Type} : RG_unlE A.
 Proof.
     exact RG_empty.
 Defined.
 
 
-Definition singleton_RG {A : Type} (a : A) : RG A.
+Definition RG_unlE_singleton {A : Type} (a : A) : RG_unlE A.
 Proof.
     refine {|
         RG_nodes := fun (x : A) => a = x;
-        RG_edges := fun x y => False;
+        RG_edges := fun x y l => False;
         RG_valid := _
     |}.
     RG_valid_prover.
 Defined.
 
 
-Definition overlay_RG {A : Type} (rg1 rg2 : RG A) : RG A.
+Definition RG_unlE_overlay {A : Type} (rg1 rg2 : RG_unlE A) : RG_unlE A.
 Proof.
     refine {|
         RG_nodes := fun A => (rg1.(RG_nodes) A) \/ (rg2.(RG_nodes) A);
-        RG_edges := fun A B => (rg1.(RG_edges) A B) \/ (rg2.(RG_edges) A B);
+        RG_edges := fun A B l => (rg1.(RG_edges) A B l) \/ (rg2.(RG_edges) A B l);
         RG_valid := _
     |}.
     RG_valid_prover_withs rg1 rg2.
@@ -34,12 +34,12 @@ Defined.
 
 
 
-Definition connect_RG {A : Type} (rg1 rg2 : RG A) : RG A.
+Definition RG_unlE_connect {A : Type} (rg1 rg2 : RG_unlE A) : RG_unlE A.
 Proof.
-    let overlay := constr:(overlay_RG rg1 rg2) in
+    let overlay := constr:(RG_unlE_overlay rg1 rg2) in
     refine {|
         RG_nodes := overlay.(RG_nodes);
-        RG_edges := fun A B => overlay.(RG_edges) A B \/ (rg1.(RG_nodes) A /\ rg2.(RG_nodes) B);
+        RG_edges := fun n1 n2 l => overlay.(RG_edges) n1 n2 l \/ (rg1.(RG_nodes) n1 /\ rg2.(RG_nodes) n2);
         RG_valid := _
     |}.
     RG_valid_prover_withs rg1 rg2.
@@ -48,20 +48,21 @@ Defined.
 
 
 
-Fixpoint AG_to_RG {A : Type} (ag : AG A) : RG A :=
+Fixpoint AG_to_RG_unlE {A : Type} (ag : AG A) : RG_unlE A :=
     match ag with
-    | Empty => empty_RG
-    | Vertex x => singleton_RG x
-    | Overlay ag1 ag2 => overlay_RG (AG_to_RG ag1) (AG_to_RG ag2)
-    | Connect ag1 ag2 => connect_RG (AG_to_RG ag1) (AG_to_RG ag2)
+    | Empty => RG_unlE_empty
+    | Vertex x => RG_unlE_singleton x
+    | Overlay ag1 ag2 => RG_unlE_overlay (AG_to_RG_unlE ag1) (AG_to_RG_unlE ag2)
+    | Connect ag1 ag2 => RG_unlE_connect (AG_to_RG_unlE ag1) (AG_to_RG_unlE ag2)
     end
 .
 
 (* TODO: this coercion may or may not be good to have *)
-Coercion AG_to_RG : AG >-> RG.
+Coercion AG_to_RG_unlE : AG >-> RG_unlE.
 
 
+(* todo: define this in terms of RG_unlE_equiv *)
 Definition AG_equiv {A : Type} (ag1 ag2 : AG A) : Prop :=
-    RG_equiv ag1 ag2.
+    RG_equiv (AG_to_RG_unlE ag1) (AG_to_RG_unlE ag2).
 
 Notation "g1 A== g2" := (AG_equiv g1 g2) (at level 80).
