project/inductive/basic/inductive_graph_basic_to_RG.v
@@ -14,17 +14,17 @@ Require Import MyProject.project.util.NatSet.
 Require Import MyProject.project.inductive.basic.inductive_graph_basic.
 Require Import MyProject.project.relational_graph.
 Require Import MyProject.project.relational_graph_theory.
-Require Import MyProject.project.relational_graph_IG_basic_operations.
+Require Import MyProject.project.relational_graph_IG_operations.
 
 
-(* Defining Conversion function from IG_basic to RG (going towards a model-based approach) *)
+(* Defining Conversion function from IG_basic to RG_unlE (going towards a model-based approach) *)
 (* Also states (and eventually proves) that operations on IG_basic are equivalent to those of RG *)
 
 
 
 (* Adds a node and its in- and out- going edges (= its IG context) to an RG.
     Assumes that the neighboring nodes exist *)
-Definition _accTo_RG (node : Node) (rgIg : RG nat * IG_basic) : RG nat * IG_basic :=
+Definition _accTo_RG_unlE (node : Node) (rgIg : RG_unlE nat * IG_basic) : RG_unlE nat * IG_basic :=
     match rgIg with | (rg, ig) =>
         match IG_basic_match node ig with
         | (Some (froms, tos), rest) => (_extendByContext node froms tos rg, rest)
@@ -33,8 +33,8 @@ Definition _accTo_RG (node : Node) (rgIg : RG nat * IG_basic) : RG nat * IG_basi
     end
 .
 
-Definition IG_basic_to_RG (ig : IG_basic) : RG nat :=
-    match fold_right _accTo_RG (RG_empty, ig) (IG_basic_labNodes ig) with
+Definition IG_basic_to_RG_unlE (ig : IG_basic) : RG_unlE nat :=
+    match fold_right _accTo_RG_unlE (RG_empty, ig) (IG_basic_labNodes ig) with
     | (rg, acc) => rg
     end
 .
@@ -43,7 +43,7 @@ Definition IG_basic_to_RG (ig : IG_basic) : RG nat :=
 (* Coercion IG_basic_to_RG : IG_basic >-> RG. *)
 
 Definition IG_basic_equiv (ig1 ig2 : IG_basic) : Prop :=
-    RG_equiv (IG_basic_to_RG ig1) (IG_basic_to_RG ig2)
+    RG_equiv (IG_basic_to_RG_unlE ig1) (IG_basic_to_RG_unlE ig2)
 .
 
 Notation "g1 I== g2" := (IG_basic_equiv g1 g2) (at level 80).
@@ -60,7 +60,7 @@ Definition IG_basic_Propify_isEmpty (result : bool) : Prop.
 Proof.
 Admitted.
 
-Definition IG_basic_Propify_matsh (result : option (NatSet.t * NatSet.t) * IG_basic) : (Prop * (Ensemble nat * Ensemble nat)) * RG nat.
+Definition IG_basic_Propify_match (result : option (NatSet.t * NatSet.t) * IG_basic) : (Prop * Context nat unit) * RG_unlE nat.
 Proof.
 Admitted.
 
@@ -70,27 +70,27 @@ Admitted.
 
 
 Theorem IG_basic_empty_relate :
-  IG_basic_to_RG IG_basic_empty = RG_empty.
+  IG_basic_to_RG_unlE IG_basic_empty = RG_empty.
 Proof.
 Admitted.
 
 Theorem IG_basic_isEmpty_relate : forall (ig : IG_basic),
-  IG_basic_Propify_isEmpty (IG_basic_isEmpty ig) = RG_isEmpty (IG_basic_to_RG ig).
+  IG_basic_Propify_isEmpty (IG_basic_isEmpty ig) = RG_isEmpty (IG_basic_to_RG_unlE ig).
 Proof.
 Admitted.
 
 
 Theorem IG_basic_match_relate : forall (node : Node) (ig : IG_basic),
-  IG_basic_Propify_matsh (IG_basic_match node ig) = RG_match node (IG_basic_to_RG ig).
+  IG_basic_Propify_match (IG_basic_match node ig) = RG_match node (IG_basic_to_RG_unlE ig).
 Proof.
 Admitted.
 
 Theorem IG_basic_mkGraph_relate : forall (nodes : list Node) (edges : list (Node * Node)),
-  IG_basic_to_RG (IG_basic_mkGraph nodes edges) = RG_mkGraph nodes edges.
+  IG_basic_to_RG_unlE (IG_basic_mkGraph nodes edges) = RG_mkGraph nodes (map (fun '(n1, n2) => (n1, n2, tt)) edges).
 Proof.
 Admitted.
 
 Theorem IG_basic_labNodes_relate : forall (ig : IG_basic),
-  IG_basic_Propify_labNodes (IG_basic_labNodes ig) = RG_labNodes (IG_basic_to_RG ig).
+  IG_basic_Propify_labNodes (IG_basic_labNodes ig) = RG_labNodes (IG_basic_to_RG_unlE ig).
 Proof.
 Admitted.
