project/relational_graph.v
@@ -9,53 +9,71 @@ Require Import MyProject.project.util.util.
 
 (* Defining a Relational Graph and its (possible) operations *)
 
+Definition _edgeRelation (A B: Type) := A -> A -> B -> Prop.
 
-Definition _valid_cond {A : Type} (nodes : Ensemble A) (edges : relation A) : Prop :=
-    forall (a1 a2 : A), edges a1 a2 -> nodes a1 /\ nodes a2.
+Definition _unlabelEdgeRelation {A B: Type} (edges : _edgeRelation A B) : relation A :=
+    fun (a1 a2 : A) => exists (l: B), edges a1 a2 l.
 
 
-Record RG (A : Type) := {
+
+(* Here, I first _temporarily_ define a more powerful RG, which has edge labels. The current RG can be derived from it *)
+
+
+Definition _valid_cond {A B: Type} (nodes : Ensemble A) (edges : _edgeRelation A B) : Prop :=
+    forall (a1 a2 : A) (b : B), edges a1 a2 b -> nodes a1 /\ nodes a2.
+
+
+Record RG (A B: Type) := {
     RG_nodes : Ensemble A;
-    RG_edges : relation A;
+    RG_edges : _edgeRelation A B;
     RG_valid : _valid_cond RG_nodes RG_edges
 }.
 
-Arguments RG_nodes {A}.
-Arguments RG_edges {A}.
-Arguments RG_valid {A}.
+
+Arguments RG_nodes {A B}.
+Arguments RG_edges {A B}.
+Arguments RG_valid {A B}.
+
 
 Ltac RG_valid_prover := unfold _valid_cond; firstorder.
 Ltac RG_valid_prover_with rg := pose proof rg.(RG_valid); RG_valid_prover.
 Ltac RG_valid_prover_withs rg1 rg2 := pose proof rg1.(RG_valid); RG_valid_prover_with rg2.
 
-
-(* Two record graphs are "the same", when their Ensemble and relation are the same *)
-Definition RG_equiv {A : Type} (rg1 rg2 : RG A) : Prop :=
+(* Two relational graphs are "the same", when their Ensemble and relation are the same *)
+Definition RG_equiv {A B : Type} (rg1 rg2 : RG A B) : Prop :=
     (* The first condition is definitely needed, as we can have "singleton" graphs *)
     (forall (a : A), rg1.(RG_nodes) a <-> rg2.(RG_nodes) a)
-    /\ (forall (a1 a2 : A), rg1.(RG_edges) a1 a2 <-> rg2.(RG_edges) a1 a2)
+    /\ (forall (a1 a2 : A) (b : B), rg1.(RG_edges) a1 a2 b <-> rg2.(RG_edges) a1 a2 b)
 .
 Notation "g1 === g2" := (RG_equiv g1 g2) (at level 100, right associativity).
 
 
+Definition RG_unlE (A : Type) := RG A unit.
+(* The followign two don't actually make sense, since one needs a node type for... well nodes to exists *)
+(* Definition RG_unlN (B : Type) := RG unit B.
+Definition RG_unl (B : Type) := RG unit unit. *)
 
-(* Defining Basic Operations on RGs: *)
 
-Definition RG_empty {A : Type} : RG A.
+
+
+(* Defining fundamental Operations on RGs: *)
+
+Definition RG_empty {A B : Type} : RG A B.
 Proof.
     refine {|
-        RG_nodes := fun A => False;
-        RG_edges := fun A B => False;
+        RG_nodes := fun a => False;
+        RG_edges := fun a1 a2 l => False;
         RG_valid := _
     |}.
     RG_valid_prover.
 Defined.
 
-Definition RG_isEmpty {A : Type} (rg : RG A) : Prop :=
+Definition RG_isEmpty {A B: Type} (rg : RG A B) : Prop :=
     forall (a : A), rg.(RG_nodes) a = False
 .
 
-Definition RG_addNode {A : Type} (node : A) (rg : RG A) : RG A.
+
+Definition RG_addNode {A B : Type} (node : A) (rg : RG A B) : RG A B.
 Proof.
     refine {|
         RG_nodes := fun a => node = a \/ rg.(RG_nodes) a;
@@ -66,11 +84,12 @@ Proof.
 Defined. 
 
 
-Definition RG_addEdge {A : Type} (from to : A) (rg : RG A) : RG A.
+Definition RG_addEdge {A B : Type} (from to : A) (label : B) (rg : RG A B) : RG A B.
 Proof.
     refine {|
         RG_nodes := fun a => (RG_addNode to (RG_addNode from rg)).(RG_nodes) a;
-        RG_edges := fun a1 a2 => (a1 = from /\ a2 = to) \/ rg.(RG_edges) a1 a2;
+        RG_edges := fun a1 a2 l =>  (a1 = from /\ a2 = to /\ l = label) \/
+                                    rg.(RG_edges) a1 a2 l;
         RG_valid := _
     |}.    
     RG_valid_prover_with rg.
@@ -78,11 +97,11 @@ Defined.
 
 
 (* Also removes all associated edges *)
-Definition RG_removeNode {A : Type} (node : A) (rg : RG A) : RG A.
+Definition RG_removeNode {A B : Type} (node : A) (rg : RG A B) : RG A B.
 Proof.
     refine {|
         RG_nodes := fun a => node <> a /\ rg.(RG_nodes) a;
-        RG_edges := fun a1 a2 => node <> a1 /\ node <> a2 /\ rg.(RG_edges) a1 a2;
+        RG_edges := fun a1 a2 l => a1 <> node /\ a2 <> node /\ rg.(RG_edges) a1 a2 l;
         RG_valid := _
     |}.
     RG_valid_prover_with rg.
@@ -90,11 +109,12 @@ Defined.
 
 
 (* Does not remove associated nodes *)
-Definition RG_removeEdge {A : Type} (from to : A) (rg : RG A) : RG A.
+Definition RG_removeEdge {A B : Type} (from to : A) (label : B) (rg : RG A B) : RG A B.
 Proof.
     refine {|
         RG_nodes := rg.(RG_nodes);
-        RG_edges := fun a1 a2 => from <> a1 /\ to <> a2 /\ rg.(RG_edges) a1 a2;
+        RG_edges := fun a1 a2 l =>  not (a1 = from /\ a2 = to /\ l = label) /\
+                                    rg.(RG_edges) a1 a2 l;
         RG_valid := _
     |}.
     RG_valid_prover_with rg.
@@ -102,14 +122,15 @@ Defined.
  
 
 
-Definition RG_getOutgoingEdges {A : Type} (node : A) (rg : RG A) : relation A :=
-    fun (a1 a2 : A) => rg.(RG_edges) a1 a2 /\ a1 = node.
+Definition RG_getOutgoingEdges {A B : Type} (node : A) (rg : RG A B) : _edgeRelation A B :=
+    fun (a1 a2 : A) l => rg.(RG_edges) a1 a2 l /\ a1 = node.
 
-Definition RG_getIncomingEdges {A : Type} (node : A) (rg : RG A) : relation A :=
-    fun (a1 a2 : A) => rg.(RG_edges) a1 a2 /\ a2 = node.
+Definition RG_getIncomingEdges {A B : Type} (node : A) (rg : RG A B) : _edgeRelation A B :=
+    fun (a1 a2 : A) l => rg.(RG_edges) a1 a2 l /\ a2 = node.
 
-Definition RG_getIncidentEdges {A : Type} (node : A) (rg : RG A) : relation A :=
-    fun (a1 a2 : A) => (RG_getOutgoingEdges node rg) a1 a2 \/ (RG_getIncomingEdges node rg) a1 a2.
+Definition RG_getIncidentEdges {A B : Type} (node : A) (rg : RG A B) : _edgeRelation A B :=
+    fun (a1 a2 : A) l =>    (RG_getOutgoingEdges node rg) a1 a2 l \/
+                            (RG_getIncomingEdges node rg) a1 a2 l.
 
 (* There can also be variations of this, where you the the neighbor nodes and not just edges ... *)
 
@@ -118,14 +139,14 @@ Definition RG_getIncidentEdges {A : Type} (node : A) (rg : RG A) : relation A :=
 (* A little exotic, but useful for IGs *)
 (* Adds a node and its in- and out- going edges (= its IG context) to an RG.
     Adds the neighbouring nodes, in case they do not exists *)
-Definition _extendByContext (node : nat) (froms tos : NatSet.t) (rg : RG nat) : RG nat.
+Definition _extendByContext (node : nat) (froms tos : NatSet.t) (rg : RG_unlE nat) : RG_unlE nat.
 Proof.
     refine {|
         RG_nodes := fun (n : nat) => NatSet.In n froms \/ NatSet.In n tos \/ (_customEnsembleAdd node rg.(RG_nodes))  n;
-        RG_edges := fun (n1 n2 : nat) =>
+        RG_edges := fun (n1 n2 : nat) l =>
                                 (NatSet.In n1 froms /\ n2 = node)
                                 \/ (n1 = node /\ NatSet.In n2 tos)
-                                \/ rg.(RG_edges) n1 n2
+                                \/ rg.(RG_edges) n1 n2 l
                                 ;
                      
         RG_valid := _
@@ -134,8 +155,8 @@ Proof.
 Defined.
 
 (* Connectedness *)
-Definition RG_existsPath {A : Type} (node1 node2 : A) (rg : RG A) : Prop :=
-    clos_trans A rg.(RG_edges) node1 node2.
+Definition RG_existsPath {A B : Type} (node1 node2 : A) (rg : RG A B) : Prop :=
+    clos_trans A (_unlabelEdgeRelation rg.(RG_edges)) node1 node2.
 
 (* Start implementing search *)
 
