project/algebraic/algebraic_graph_theory.v
@@ -76,7 +76,7 @@ Qed.
 (* This proof is based on === being an equivalence relation *)
 Instance AG_Equivalence_eq {A : Type} : Equivalence (@AG_equiv A).
 Proof.
-    G_derived_equivalence_prover A (@AG_to_RG A).
+    G_derived_equivalence_prover A unit (@AG_to_RG_unlE A).
 Qed.
          
 
