project/relational_graph_theory.v
@@ -8,20 +8,20 @@ Require Import MyProject.project.relational_graph.
 
 (* "RG_equiv" is an equivalence relation: *)
 (* Reflexive *)
-Theorem RG_equiv_Reflexive {A : Type}: forall (rg : RG A), RG_equiv rg rg.
+Theorem RG_equiv_Reflexive {A B : Type}: forall (rg : RG A B), RG_equiv rg rg.
 Proof.
     firstorder.
 Qed.
     
 
 (* Symmetric *)
-Theorem RG_equiv_Symmetric {A : Type}: forall (rg1 rg2 : RG A), RG_equiv rg1 rg2 <-> RG_equiv rg2 rg1.
+Theorem RG_equiv_Symmetric {A B : Type}: forall (rg1 rg2 : RG A B), RG_equiv rg1 rg2 <-> RG_equiv rg2 rg1.
 Proof.
     firstorder.
 Qed. 
 
 (* Transitive *)
-Theorem RG_equiv_Transitive {A : Type}: forall (rg1 rg2 rg3 : RG A), RG_equiv rg1 rg2 -> RG_equiv rg2 rg3 -> RG_equiv rg1 rg3.
+Theorem RG_equiv_Transitive {A B : Type}: forall (rg1 rg2 rg3 : RG A B), RG_equiv rg1 rg2 -> RG_equiv rg2 rg3 -> RG_equiv rg1 rg3.
 Proof.
     firstorder.
     - apply H1. apply H2. apply H3.
@@ -32,19 +32,19 @@ Qed.
 
 (* Source for rewrite: https://stackoverflow.com/questions/56099646/use-rewrite-tactic-with-my-own-operator-in-coq *)
 Require Import Setoid Morphisms.
-Instance RG_Equivalence_eq {A : Type} : Equivalence (@RG_equiv A).
+Instance RG_Equivalence_eq {A B : Type} : Equivalence (@RG_equiv A B).
 Proof.
     unfold RG_equiv. split.
     - unfold Reflexive. intros. pose proof (@RG_equiv_Reflexive A). apply H.
     - unfold Symmetric. intros. pose proof (@RG_equiv_Symmetric A). apply H0. apply H.
-    - unfold Transitive. intros. pose proof (@RG_equiv_Transitive A). apply (H1 x y).
+    - unfold Transitive. intros. pose proof (@RG_equiv_Transitive A B). apply (H1 x y).
         + apply H.
         + apply H0.
 Qed.
 
 (* Does something very similar as the proof above, but uses "other evidence" for equivalence *)
-Ltac G_derived_equivalence_prover A f :=
-  pose proof (@RG_Equivalence_eq A) as H;
+Ltac G_derived_equivalence_prover A B f :=
+  pose proof (@RG_Equivalence_eq A B) as H;
   destruct H as [Eq_Refl Eq_Symm Eq_Trans]; split;
   [ unfold Reflexive; intros; unfold Reflexive in Eq_Refl; apply Eq_Refl
   | unfold Symmetric; intros; unfold Symmetric in Eq_Symm; apply Eq_Symm; apply H
